term.v
@@ -149,23 +149,25 @@ Fixpoint nonces_of_term t : gset loc :=
 
 Module Spec.
 
-Definition tag_def (c : string) (t : term) :=
-  TPair (TInt (Zpos (encode c))) t.
+Implicit Types N : namespace.
+
+Definition tag_def N (t : term) :=
+  TPair (TInt (Zpos (encode N))) t.
 Definition tag_aux : seal tag_def. by eexists. Qed.
 Definition tag := unseal tag_aux.
 Lemma tag_eq : tag = tag_def. Proof. exact: seal_eq. Qed.
 
-Definition untag_def (c : string) (t : term) :=
+Definition untag_def N (t : term) :=
   match t with
   | TPair (TInt (Zpos m)) t =>
-    if decide (encode c = m) then Some t else None
+    if decide (encode N = m) then Some t else None
   | _ => None
   end.
 Definition untag_aux : seal untag_def. by eexists. Qed.
 Definition untag := unseal untag_aux.
 Lemma untag_eq : untag = untag_def. Proof. exact: seal_eq. Qed.
 
-Lemma tagK c t : untag c (tag c t) = Some t.
+Lemma tagK N t : untag N (tag N t) = Some t.
 Proof.
 rewrite untag_eq tag_eq /untag_def /tag_def /=.
 by rewrite decide_left.
@@ -177,9 +179,9 @@ rewrite tag_eq /tag_def => c1 t1 c2 t2 [] e ->.
 split=> //; by apply: inj e.
 Qed.
 
-Lemma untagK c t1 t2 :
-  untag c t1 = Some t2 ->
-  t1 = tag c t2.
+Lemma untagK N t1 t2 :
+  untag N t1 = Some t2 ->
+  t1 = tag N t2.
 Proof.
 rewrite untag_eq tag_eq /=.
 case: t1=> [] // [] // [] //= m.
